# Recursive Algorithms

## Running Time

- `T(n)` can be expressed as recurrence
  - `T(n) = T(n - 1) + cn`
  - `T(1) = c`
- 1 recursive call on problem with one less value `+`
- `Œ∏(n)` recursive steps

### Recursive Analysis Example

```text
T(n) = T(n - 1) + c‚ÇÅn
T(1) = c‚ÇÇ
```

- Find expression for `T(n - 1)`

```text
T(n - 1) = T((n - 1) - 1) + c‚ÇÅ(n - 1)
T(n - 1) = T(n - 2) + c‚ÇÅ(n - 1)
```

- Then put that exp. into the original equation

```text
T(n) = T(n - 2) + c‚ÇÅ(n - 1) + c‚ÇÅn
T(n) = T(n - 2) + c‚ÇÅn - c‚ÇÅ + c‚ÇÅn
T(n) = T(n - 2) + 2c‚ÇÅn - c‚ÇÅ
```

- Repeat until pattern is found

```text
T(n - 2) = T((n - 2) - 1) + c‚ÇÅ(n - 2)
T(n - 2) = T(n - 3) + c‚ÇÅ(n - 2)
```

- And put it in the original ...

```text
T(n) = T(n - 3) + c‚ÇÅ(n - 2) + 2c‚ÇÅn - c‚ÇÅ
T(n) = T(n - 3) + c‚ÇÅn - 2c‚ÇÅ + 2c‚ÇÅn - c‚ÇÅ
T(n) = T(n - 3) + 3c‚ÇÅn - 3c‚ÇÅ
```

- And another one ...

```text
T(n - 3) = T((n - 3) - 1) + c‚ÇÅ(n - 3)
T(n - 3) = T(n - 4) + c‚ÇÅ(n - 3)
```

- You know the deal by now üòâ

```text
T(n) = T(n - 4) + c‚ÇÅ(n - 3) + 3c‚ÇÅn - 3c‚ÇÅ
T(n) = T(n - 4) + c‚ÇÅn - 3c‚ÇÅ + 3c‚ÇÅn - 3c‚ÇÅ
T(n) = T(n - 4) + 4c‚ÇÅn - 6c‚ÇÅ
```

- The stages of `T(n)`

```text
T(n) = T(n - 1) + 1c‚ÇÅn - 0c‚ÇÅ
T(n) = T(n - 2) + 2c‚ÇÅn - 1c‚ÇÅ
T(n) = T(n - 3) + 3c‚ÇÅn - 3c‚ÇÅ
T(n) = T(n - 4) + 4c‚ÇÅn - 6c‚ÇÅ
T(n) = T(n - 5) + 5c‚ÇÅn - 10c‚ÇÅ
```

- The equation:

```text
T(n) = T(n - k) + kc‚ÇÅn - (k * (k + 1) / 2)c‚ÇÅ
```

- Considering the base case so `k` is `n - 1` with the base case as `T(1) = c‚ÇÇ`

```text
T(n) = T(n - k) + kc‚ÇÅn - (k * (k + 1) / 2)c‚ÇÅ
T(n) = T(n - (n - 1)) + (n - 1)c‚ÇÅn - ((n - 1) * ((n - 1) + 1) / 2)c‚ÇÅ
T(n) = T(1) + (c‚ÇÅn¬≤ - c‚ÇÅn) - ((n - 1) * n / 2)c‚ÇÅ
T(n) = c‚ÇÇ + c‚ÇÅn¬≤ - c‚ÇÅn - ((n¬≤ - n) / 2)c‚ÇÅ
T(n) = c‚ÇÇ + c‚ÇÅn¬≤ - c‚ÇÅn - ¬Ωn¬≤c‚ÇÅ + ¬Ωnc‚ÇÅ
T(n) = c‚ÇÇ + ¬Ωn¬≤c‚ÇÅ - ¬Ωnc‚ÇÅ
```

- So this example has a running time complexity of `Œ∏(n¬≤)`
